Reduce docker image size; Adapt examples to changes in the preliminary HTTP layer

workspace/src/cat-fact-api/DY.CatFactAPI.Protocol.fst
@@ -27,21 +27,21 @@ instance local_state_state_t: local_state state_t = {
   format = parseable_serializeable_bytes_state_t;
 }
 
-val api_request: communication_keys_sess_ids -> principal -> principal -> traceful (option (state_id & timestamp))
-let api_request comm_keys_ids client server =
-  let u:url kv_types = {
-    protocol = "https";
-    domain = {root_domain = server; sub_domain = ""};
+val api_request: communication_keys_sess_ids -> principal -> traceful (option (state_id & timestamp))
+let api_request comm_keys_ids client =
+  let url:url_t kv_types = {
+    protocol = HTTPS;
+    domain = ["catfact"; "ninja"];
     port = 443;
     path = "/fact";
     query = [{ key = "max_length"; value = VI 140 } <: key_value kv_types];
     fragment = {identifier = ""; data = []};
   } in
-  let headers:list (header kv_types) = [
+  let headers:list (header_t kv_types) = [
     Accept "application/json";
   ] in
-  let http_req = mk_http_request GET u headers empty_body in
-  let*? (msg_id, hmeta_data) = send_https_request comm_keys_ids client u http_req in
+  let http_req = mk_http_request GET url headers empty_body in
+  let*? (msg_id, hmeta_data) = send_https_request comm_keys_ids client url http_req in
 
   let* sid = new_session_id client in
   set_state client sid (SendRequest hmeta_data);*
@@ -50,7 +50,7 @@ let api_request comm_keys_ids client server =
 val api_server: communication_keys_sess_ids -> principal -> timestamp -> traceful (option timestamp)
 let api_server comm_keys_ids server msg_id =
   let*? (http_req, hmeta_data) = receive_https_request comm_keys_ids server msg_id in
-  let headers:list (header kv_types) = [ContentType "application/json"] in
+  let headers:list (header_t kv_types) = [ContentType "application/json"] in
   let body = JSON [{key = "fact"; value = VS "Cats are great!"}; {key="length"; value=VI 15}] in
   let http_res = mk_http_response 200 headers body in
   let*? msg_id_out = send_https_response server hmeta_data http_res in
@@ -59,7 +59,7 @@ let api_server comm_keys_ids server msg_id =
 val api_response: principal -> state_id -> timestamp -> traceful (option unit)
 let api_response client sid msg_id =
   let*? SendRequest hmeta_data = get_state client sid in
-  let*? (http_res, hmeta_data) = receive_https_response hmeta_data client msg_id in
+  let*? http_res = receive_https_response hmeta_data client msg_id in
   let*? fact = return (get_string_from_json_encoded "fact" http_res.body) in
   let _ = IO.debug_print_string (Printf.sprintf "\nReceived fact: %s\n\n" fact) in
   return (Some ())
