workspace/src/potter-api/DY.PotterAPI.Extraction.fst
@@ -13,7 +13,7 @@ let run () : traceful (option unit)  =
   let client:principal = "Alice" in
   let server:principal = "potterapi-fedeperin.vercel.app" in
 
-  let*? comm_keys_ids_client, comm_keys_ids_server = initialize_communication_reqres (http web_types kv_types) client server in
+  let*? comm_keys_ids_client, comm_keys_ids_server = initialize_communication_reqres (http_t web_types kv_types) client server in
   
   let*? sid, msg_id = api_request comm_keys_ids_client client server in
   let*? () = api_response client sid msg_id in
