workspace/src/potter-api/DY.PotterAPI.Protocol.fst
@@ -29,9 +29,9 @@ instance local_state_state_t: local_state state_t = {
 
 val api_request: communication_keys_sess_ids -> principal -> principal -> traceful (option (state_id & timestamp))
 let api_request comm_keys_ids client server =
-  let u:url kv_types = {
-    protocol = "https";
-    domain = {root_domain = server; sub_domain = ""};
+  let u:url_t kv_types = {
+    protocol = HTTPS;
+    domain = ["potterapi-fedeperin"; "vercel"; "app"];
     port = 443;
     path = "/en/spells/random";
     query = [];
@@ -50,7 +50,7 @@ let api_request comm_keys_ids client server =
 val api_server: communication_keys_sess_ids -> principal -> timestamp -> traceful (option timestamp)
 let api_server comm_keys_ids server msg_id =
   let*? (http_req, hmeta_data) = receive_https_request comm_keys_ids server msg_id in
-  let headers:list (header kv_types) = [ContentType "application/json"] in
+  let headers:list (header_t kv_types) = [ContentType "application/json"] in
   let body = JSON [{key = "spell"; value = VS "Prior Incantato" }; {key = "use"; value = VS "Reveals last spell cast" }; {key =  "index"; value = VI 29}] in
   let http_res = mk_http_response 200 headers body in
   let*? msg_id_out = send_https_response server hmeta_data http_res in
@@ -59,7 +59,7 @@ let api_server comm_keys_ids server msg_id =
 val api_response: principal -> state_id -> timestamp -> traceful (option unit)
 let api_response client sid msg_id =
   let*? SendRequest hmeta_data = get_state client sid in
-  let*? (http_res, hmeta_data) = receive_https_response hmeta_data client msg_id in
+  let*? http_res = receive_https_response hmeta_data client msg_id in
   let*? spell = return (get_string_from_json_encoded "spell" http_res.body) in
   let _ = IO.debug_print_string (Printf.sprintf "\nReceived spell: %s\n" spell) in
   let*? use = return (get_string_from_json_encoded "use" http_res.body) in
